Prove some more head lemmas

candle/prover/candle_kernel_valsScript.sml
@@ -235,6 +235,14 @@ Definition PAIR_TYPE_HEAD_def:
   PAIR_TYPE_HEAD h1 h2 v = PAIR_TYPE (K h1) (K h2) ((),()) v
 End
 
+Definition STRING_TYPE_HEAD_def:
+  STRING_TYPE_HEAD v ⇔ ∃s. STRING_TYPE s v
+End
+
+Definition NUM_HEAD_def:
+  NUM_HEAD v ⇔ ∃n. NUM n v
+End
+
 (* -------------------------------------------------------------------------
  * THM, TERM, TYPE lemmas
  * ------------------------------------------------------------------------- *)
@@ -341,6 +349,20 @@ Proof
   \\ rename [‘Conv oo ll’] \\ Cases_on ‘oo’ \\ gvs [pmatch_def,AllCaseEqs()]
 QED
 
+Theorem evaluate_str_check:
+  evaluate ^s env
+    [Let NONE (App Strlen [Var (Short v)]) ee] = (s',res) ∧
+  nsLookup env.v (Short v) = SOME w ⇒
+  ^safe_error_goal ∨ STRING_TYPE_HEAD w ∧ evaluate ^s env [ee] = (s',res)
+Proof
+  fs [evaluate_def,same_ctor_def,pmatch_def,do_con_check_def] \\ csimp []
+  \\ fs [do_app_def,AllCaseEqs()] \\ strip_tac \\ gvs [same_clock_exists]
+  \\ fs [STRING_TYPE_HEAD_def,STRING_TYPE_def,namespaceTheory.nsOptBind_def]
+  \\ last_x_assum (rewrite_tac o single o GSYM)
+  \\ disj2_tac \\ rpt (AP_THM_TAC ORELSE AP_TERM_TAC)
+  \\ fs [state_component_equality]
+QED
+
 Theorem evaluate_ty_check:
   evaluate ^s env
     [Let NONE
@@ -394,6 +416,51 @@ Proof
   \\ CONV_TAC (DEPTH_CONV ml_progLib.nsLookup_conv) \\ simp []
   \\ fs [namespaceTheory.nsOptBind_def]
 QED
+
+Theorem evaluate_mat_pair:
+  evaluate ^s env
+    [Mat (Var (Short v)) [(Pcon NONE [Pvar a1; Pvar a2], ee)]] = (s',res) ∧
+  nsLookup env.v (Short v) = SOME w ⇒
+  ^safe_error_goal ∨
+  ∃v1 v2.
+    w = Conv NONE [v1;v2] ∧
+    evaluate s (env with v := nsBind a2 v2 (nsBind a1 v1 env.v)) [ee] = (s',res)
+Proof
+  fs [evaluate_def,same_ctor_def,pmatch_def,do_con_check_def] \\ csimp []
+  \\ rpt strip_tac
+  \\ gvs [AllCaseEqs(),LENGTH_EQ_NUM_compute,same_clock_exists]
+  \\ Cases_on ‘w’ \\ gvs [pmatch_def]
+  \\ rename [‘Conv oo ll’] \\ Cases_on ‘oo’ \\ gvs [pmatch_def,AllCaseEqs()]
+  \\ gvs [AllCaseEqs(),LENGTH_EQ_NUM_compute,pmatch_def]
+QED
+
+
+(*
+Theorem evaluate_mat_thm:
+  evaluate ^s env
+    [Mat (Var (Short v))
+       [(Pcon (SOME (Short "Sequent")) [Pvar a1], ee)]] = (s',res) ∧
+  nsLookup env.c (Short "Sequent") = SOME (2,TypeStamp "Sequent" thm_stamp_n) ∧
+  nsLookup env.v (Short v) = SOME w ⇒
+  ^safe_error_goal ∨ THM_TYPE_HEAD w ∧ evaluate ^s env [ee] = (s',res)
+Proof
+  fs [evaluate_def,same_ctor_def,pmatch_def,do_con_check_def] \\ csimp []
+  \\ CONV_TAC (DEPTH_CONV ml_progLib.nsLookup_conv) \\ simp []
+  \\ rpt strip_tac
+  \\ gvs [AllCaseEqs(),LENGTH_EQ_NUM_compute,same_clock_exists]
+  \\ Cases_on ‘w’ \\ gvs [pmatch_def]
+  \\ rename [‘Conv oo ll’] \\ Cases_on ‘oo’ \\ gvs [pmatch_def,AllCaseEqs()]
+  \\ gvs [AllCaseEqs(),LENGTH_EQ_NUM_compute]
+  \\ rpt strip_tac \\ gvs [same_ctor_def,pmatch_def]
+  \\ fs [THM_TYPE_HEAD_def]
+
+
+
+  \\ rpt (pop_assum mp_tac)
+  \\ CONV_TAC (DEPTH_CONV ml_progLib.nsLookup_conv) \\ simp []
+  \\ fs [namespaceTheory.nsOptBind_def]
+QED
+*)
 
 Theorem is_type_v_head:
   do_opapp [is_type_v; w] = SOME (env, exp) ∧
@@ -812,6 +879,70 @@ Proof
   \\ fs [] \\ CONV_TAC (DEPTH_CONV ml_progLib.nsLookup_conv) \\ simp []
 QED
 
+Theorem evaluate_ty_list_check:
+  evaluate ^s env
+    [Let NONE (App Opapp [Var (Short "check_ty"); Var (Short v)]) ee] = (s',res) ∧
+  nsLookup env.v (Short "check_ty") = SOME check_ty_v ∧
+  nsLookup env.v (Short v) = SOME w ⇒
+  ^safe_error_goal ∨
+  LIST_TYPE_HEAD TYPE_TYPE_HEAD w ∧
+  ∃k. evaluate (^s with clock := k) env [ee] = (s',res)
+Proof
+  fs [evaluate_def,same_ctor_def,pmatch_def,do_con_check_def] \\ csimp []
+  \\ fs [do_app_def,AllCaseEqs()] \\ strip_tac \\ gvs [same_clock_exists]
+  \\ fs [STRING_TYPE_HEAD_def,STRING_TYPE_def,namespaceTheory.nsOptBind_def]
+  \\ qspecl_then [‘w’,‘s’] mp_tac check_ty_head
+  \\ fs [] \\ strip_tac \\ gvs [] \\ metis_tac []
+QED
+
+Theorem evaluate_ty_ty_list_check:
+  evaluate ^s env
+    [Let NONE (App Opapp [Var (Short "check_ty_ty"); Var (Short v)]) ee] = (s',res) ∧
+  nsLookup env.v (Short "check_ty_ty") = SOME check_ty_ty_v ∧
+  nsLookup env.v (Short v) = SOME w ⇒
+  ^safe_error_goal ∨
+  LIST_TYPE_HEAD (PAIR_TYPE_HEAD TYPE_TYPE_HEAD TYPE_TYPE_HEAD) w ∧
+  ∃k. evaluate (^s with clock := k) env [ee] = (s',res)
+Proof
+  fs [evaluate_def,same_ctor_def,pmatch_def,do_con_check_def] \\ csimp []
+  \\ fs [do_app_def,AllCaseEqs()] \\ strip_tac \\ gvs [same_clock_exists]
+  \\ fs [STRING_TYPE_HEAD_def,STRING_TYPE_def,namespaceTheory.nsOptBind_def]
+  \\ qspecl_then [‘w’,‘s’] mp_tac check_ty_ty_head
+  \\ fs [] \\ strip_tac \\ gvs [] \\ metis_tac []
+QED
+
+Theorem evaluate_tm_list_check:
+  evaluate ^s env
+    [Let NONE (App Opapp [Var (Short "check_tm"); Var (Short v)]) ee] = (s',res) ∧
+  nsLookup env.v (Short "check_tm") = SOME check_tm_v ∧
+  nsLookup env.v (Short v) = SOME w ⇒
+  ^safe_error_goal ∨
+  LIST_TYPE_HEAD TERM_TYPE_HEAD w ∧
+  ∃k. evaluate (^s with clock := k) env [ee] = (s',res)
+Proof
+  fs [evaluate_def,same_ctor_def,pmatch_def,do_con_check_def] \\ csimp []
+  \\ fs [do_app_def,AllCaseEqs()] \\ strip_tac \\ gvs [same_clock_exists]
+  \\ fs [STRING_TYPE_HEAD_def,STRING_TYPE_def,namespaceTheory.nsOptBind_def]
+  \\ qspecl_then [‘w’,‘s’] mp_tac check_tm_head
+  \\ fs [] \\ strip_tac \\ gvs [] \\ metis_tac []
+QED
+
+Theorem evaluate_tm_tm_list_check:
+  evaluate ^s env
+    [Let NONE (App Opapp [Var (Short "check_tm_tm"); Var (Short v)]) ee] = (s',res) ∧
+  nsLookup env.v (Short "check_tm_tm") = SOME check_tm_tm_v ∧
+  nsLookup env.v (Short v) = SOME w ⇒
+  ^safe_error_goal ∨
+  LIST_TYPE_HEAD (PAIR_TYPE_HEAD TERM_TYPE_HEAD TERM_TYPE_HEAD) w ∧
+  ∃k. evaluate (^s with clock := k) env [ee] = (s',res)
+Proof
+  fs [evaluate_def,same_ctor_def,pmatch_def,do_con_check_def] \\ csimp []
+  \\ fs [do_app_def,AllCaseEqs()] \\ strip_tac \\ gvs [same_clock_exists]
+  \\ fs [STRING_TYPE_HEAD_def,STRING_TYPE_def,namespaceTheory.nsOptBind_def]
+  \\ qspecl_then [‘w’,‘s’] mp_tac check_tm_tm_head
+  \\ fs [] \\ strip_tac \\ gvs [] \\ metis_tac []
+QED
+
 Theorem vsubst_v_head:
   do_partial_app vsubst_v v = SOME g ∧
   do_opapp [g; w] = SOME (env, exp) ∧
@@ -961,10 +1092,19 @@ QED
 val one_arg_tm_or_ty_tac =
   rewrite_tac[kernel_funs_v_def,do_opapp_clos]
   \\ strip_tac \\ rveq \\ fs []
-  \\ (dxrule evaluate_ty_check ORELSE dxrule evaluate_tm_check)
-  \\ simp [ml_progTheory.nsLookup_nsBind_compute]
-  \\ CONV_TAC (DEPTH_CONV ml_progLib.nsLookup_conv) \\ simp []
-  \\ strip_tac \\ simp [same_clock_exists];
+  \\ rpt (
+    (dxrule evaluate_ty_check ORELSE
+     dxrule evaluate_ty_list_check ORELSE
+     dxrule evaluate_ty_ty_list_check ORELSE
+     dxrule evaluate_tm_check ORELSE
+     dxrule evaluate_tm_list_check ORELSE
+     dxrule evaluate_tm_tm_list_check ORELSE
+     dxrule evaluate_str_check ORELSE
+     dxrule evaluate_mat_pair)
+    \\ simp [ml_progTheory.nsLookup_nsBind_compute]
+    \\ CONV_TAC (DEPTH_CONV ml_progLib.nsLookup_conv) \\ simp []
+    \\ rpt strip_tac \\ simp [same_clock_exists])
+  \\ fs [PAIR_TYPE_HEAD_def,PAIR_TYPE_def];
 
 Theorem dest_type_v_head:
   do_opapp [dest_type_v; v] = SOME (env, exp) ∧
@@ -1110,6 +1250,144 @@ Proof
   one_arg_tm_or_ty_tac
 QED
 
+Theorem call_tyvars_v_head:
+  do_opapp [call_tyvars_v; v] = SOME (env, exp) ∧
+  evaluate ^s env [exp] = (s', res) ⇒
+    ^safe_error_goal ∨
+    TYPE_TYPE_HEAD v
+Proof
+  one_arg_tm_or_ty_tac
+QED
+
+Theorem call_type_vars_in_term_v_head:
+  do_opapp [call_type_vars_in_term_v; v] = SOME (env, exp) ∧
+  evaluate ^s env [exp] = (s', res) ⇒
+    ^safe_error_goal ∨
+    TERM_TYPE_HEAD v
+Proof
+  one_arg_tm_or_ty_tac
+QED
+
+Theorem call_type_vars_in_term_v_head:
+  do_opapp [call_type_vars_in_term_v; v] = SOME (env, exp) ∧
+  evaluate ^s env [exp] = (s', res) ⇒
+    ^safe_error_goal ∨
+    TERM_TYPE_HEAD v
+Proof
+  one_arg_tm_or_ty_tac
+QED
+
+Theorem new_basic_definition_v_head:
+  do_opapp [new_basic_definition_v; v] = SOME (env, exp) ∧
+  evaluate ^s env [exp] = (s', res) ⇒
+    ^safe_error_goal ∨
+    TERM_TYPE_HEAD v
+Proof
+  one_arg_tm_or_ty_tac
+QED
+
+Theorem get_const_type_v_head:
+  do_opapp [get_const_type_v; v] = SOME (env, exp) ∧
+  evaluate ^s env [exp] = (s', res) ⇒
+    ^safe_error_goal ∨
+    STRING_TYPE_HEAD v
+Proof
+  one_arg_tm_or_ty_tac
+QED
+
+Theorem new_constant_v_head:
+  do_opapp [new_constant_v; v] = SOME (env, exp) ∧
+  evaluate ^s env [exp] = (s', res) ⇒
+    ^safe_error_goal ∨
+    PAIR_TYPE_HEAD STRING_TYPE_HEAD TYPE_TYPE_HEAD v
+Proof
+  one_arg_tm_or_ty_tac
+QED
+
+Theorem mk_var_v_head:
+  do_opapp [mk_var_v; v] = SOME (env, exp) ∧
+  evaluate ^s env [exp] = (s', res) ⇒
+    ^safe_error_goal ∨
+    PAIR_TYPE_HEAD STRING_TYPE_HEAD TYPE_TYPE_HEAD v
+Proof
+  one_arg_tm_or_ty_tac
+QED
+
+Theorem mk_comb_v_head:
+  do_opapp [mk_comb_v; v] = SOME (env, exp) ∧
+  evaluate ^s env [exp] = (s', res) ⇒
+    ^safe_error_goal ∨
+    PAIR_TYPE_HEAD TERM_TYPE_HEAD TERM_TYPE_HEAD v
+Proof
+  one_arg_tm_or_ty_tac
+QED
+
+Theorem get_type_arity_v_head:
+  do_opapp [get_type_arity_v; v] = SOME (env, exp) ∧
+  evaluate ^s env [exp] = (s', res) ⇒
+    ^safe_error_goal ∨
+    STRING_TYPE_HEAD v
+Proof
+  one_arg_tm_or_ty_tac
+QED
+
+Theorem mk_type_v_head:
+  do_opapp [mk_type_v; v] = SOME (env, exp) ∧
+  evaluate ^s env [exp] = (s', res) ⇒
+    ^safe_error_goal ∨
+    PAIR_TYPE_HEAD STRING_TYPE_HEAD (LIST_TYPE_HEAD TYPE_TYPE_HEAD) v
+Proof
+  one_arg_tm_or_ty_tac
+QED
+
+Theorem refl_v_head:
+  do_opapp [refl_v; v] = SOME (env, exp) ∧
+  evaluate ^s env [exp] = (s', res) ⇒
+    ^safe_error_goal ∨
+    TERM_TYPE_HEAD v
+Proof
+  one_arg_tm_or_ty_tac
+QED
+
+Theorem mk_const_v_head:
+  do_opapp [mk_const_v; v] = SOME (env, exp) ∧
+  evaluate ^s env [exp] = (s', res) ⇒
+    ^safe_error_goal ∨
+    PAIR_TYPE_HEAD STRING_TYPE_HEAD
+      (LIST_TYPE_HEAD (PAIR_TYPE_HEAD TYPE_TYPE_HEAD TYPE_TYPE_HEAD)) v
+Proof
+  one_arg_tm_or_ty_tac
+QED
+
+Theorem freesl_v_head:
+  do_opapp [freesl_v; v] = SOME (env, exp) ∧
+  evaluate ^s env [exp] = (s', res) ⇒
+    ^safe_error_goal ∨
+    LIST_TYPE_HEAD TERM_TYPE_HEAD v
+Proof
+  one_arg_tm_or_ty_tac
+QED
+
+Theorem assume_v_head:
+  do_opapp [assume_v; v] = SOME (env, exp) ∧
+  evaluate ^s env [exp] = (s', res) ⇒
+    ^safe_error_goal ∨
+    TERM_TYPE_HEAD v
+Proof
+  one_arg_tm_or_ty_tac
+QED
+
+(*
+Theorem hyp_v_head:
+  do_opapp [hyp_v; v] = SOME (env, exp) ∧
+  evaluate ^s env [exp] = (s', res) ⇒
+    ^safe_error_goal ∨
+    TERM_TYPE_HEAD v
+Proof
+  one_arg_tm_or_ty_tac
+QED
+*)
+
 (*
 
 Note: these head theorems should be proved as much as possible using
@@ -1117,38 +1395,29 @@ only drule with generic lemmas like evaluate_ty_check,
 evaluate_tm_check etc.
 
 TODO:
-  mk_type_v_def
-  call_type_of_v_def
-  mk_comb_1_v_def
-  get_type_arity_v
-  new_type_v
-  call_tyvars_v
-  get_const_type_v
-  new_constant_v
-  mk_var_v
-  mk_const_v
-  mk_abs_v
-  mk_comb_v
-  call_frees_v
-  freesl_v
-  call_type_vars_in_term_v
-  dest_thm_v
-  hyp_v
-  refl_v
-  assume_v
-  new_axiom_v
-  new_basic_definition_v
-  new_basic_type_definition_v
-  call_type_subst_v
-  call_freesin_v
-  call_vfree_in_v
-  vsubst_v
-  inst_v
-  abs_1_v
-  eq_mp_v
-  deduct_antisym_rule_v
-  inst_type_v
-  inst_1_v
+  hyp_v_thm
+  dest_thm_v_thm
+  mk_comb_1_v_thm
+  new_basic_type_definition_v_thm
+
+TWO ARG:
+  call_type_subst_v_thm
+  call_freesin_v_thm
+  vsubst_v_thm
+  inst_v_thm
+  abs_1_v_thm
+  eq_mp_v_thm
+  deduct_antisym_rule_v_thm
+  inst_type_v_thm
+  inst_1_v_thm
+
+FIX:
+  new_axiom_v_thm
+  mk_abs_v_thm
+  call_frees_v_thm
+  call_type_of_v_thm
+  call_vfree_in_v_thm
+  new_type_v_thm
 
 *)
 
